

• Suppose $T: V \rightarrow W$ is a linear transformation.

Recall, there is a special vector $\vec{0} = \vec{0}_W \in W$. (we will use $\vec{0}$ for the zero vector in V and W).

Suppose $x, y \in V$ are such that

$$T(x) = \vec{0} \quad \text{and} \quad T(y) = \vec{0}.$$

$$\text{Then: } T(x + y) = T(x) + T(y) = \vec{0} + \vec{0} = \vec{0}.$$

$$\text{and } T(\lambda x) = \lambda T(x) = \lambda \cdot \vec{0} = \vec{0} \quad \text{for all } \lambda \in \mathbb{F}.$$

Theorem: The kernel of $T: V \rightarrow W$ is the subspace:

$$\ker T = \left\{ x \in V \mid T(x) = \vec{0} \right\} \subset V.$$

Ex: Let $T: \mathbb{R}^2 \rightarrow \mathbb{R}$ be defined by:

$$T(a_1, a_2) = a_1$$

$$\text{Then } \ker T = \left\{ (a_1, a_2) \mid T(a_1, a_2) = \vec{0} \right\}$$

$$= \left\{ (a_1, a_2) \mid a_1 = 0 \right\} \text{ "y-axis".}$$

$$= \text{span} \{ e_2 \}.$$

• Suppose $z, w \in W$ are such that

$$z = T(x), \quad w = T(y).$$

for some $x, y \in V$. Then

$$z + w = T(x) + T(y) = T(x + y).$$

$$\text{Similarly: } \lambda z = \lambda T(x) = T(\lambda x).$$

Thus, we see that the set of vectors in the image of T is a subspace.

Theorem: The image of $T: V \rightarrow W$ is the subspace

$$\text{Im } T = \left\{ z \in W \mid \begin{array}{l} T(x) = z \\ \text{for some } x \in V. \end{array} \right\} \subset W.$$

Ex: Define $T: \mathbb{R} \rightarrow \mathbb{R}^3$ by

$$T(a) = (a, a, a)$$

Then

$$\text{Im } T = \text{span} \left\{ (1, 1, 1) \right\} = \text{span} \left\{ \begin{bmatrix} 1 \\ 1 \\ 1 \end{bmatrix} \right\}$$

A line.

Theorem : Let $T: V \rightarrow W$ be linear and $\{v_i\}_{i=1}^n$ is a basis for V . Then

$$\{T(v_i)\}_{i=1}^n$$

generates $\text{Im } T$.

Pf : Clearly $T(v_i) \in \text{Im } T$ for each i . Sp
 $w \in \text{Im } T$ is arbitrary vector in image. Then
we can find $v \in V$ s.t. $T(v) = w$.

Since $\{v_i\}$ is basis for V we can find

$$\lambda_1, \dots, \lambda_n \text{ s.t. } v = \lambda_1 v_1 + \dots + \lambda_n v_n.$$

But then

$$\begin{aligned} w = T(v) &= T(\lambda_1 v_1 + \dots + \lambda_n v_n) \\ &= \lambda_1 T(v_1) + \dots + \lambda_n T(v_n). \end{aligned}$$

$$\Rightarrow w \in \text{span} \{T(v_1), \dots, T(v_n)\}.$$

□

Ex: Let $T: P_2 \rightarrow \mathbb{R}^3$ be defined as

$$T(f) = \begin{bmatrix} f(1) - f(2) \\ 0 \\ f(0) \end{bmatrix}.$$

Since $\{1, x, x^2\}$ is basis for P_2 we know by the theorem that

$$\text{Im } T = \text{Span} \{T(1), T(x), T(x^2)\}$$

$$= \text{Span} \left\{ \begin{bmatrix} 0 \\ 0 \\ 1 \end{bmatrix}, \begin{bmatrix} -1 \\ 0 \\ 0 \end{bmatrix}, \begin{bmatrix} -3 \\ 0 \\ 0 \end{bmatrix} \right\}$$

$$= \text{Span} \left\{ \begin{bmatrix} 1 \\ 0 \\ 0 \end{bmatrix}, \begin{bmatrix} 0 \\ 0 \\ 1 \end{bmatrix} \right\} = \{xz\text{-plane}\}.$$

In particular, $\dim \text{Im } T = 2$.

• What's $\ker T$? Suppose

$$f = a + bx + cx^2 \in \ker T.$$

Then $f(1) = f(2)$ and $f(0) = 0$. So:

$$a + b + c = a + 2b + 4c \quad \text{and}$$

$$\Rightarrow \begin{matrix} a = 0 \\ b + c = 2b + 4c \end{matrix} \Rightarrow \boxed{\begin{matrix} a = 0 \\ b = -3c \end{matrix}}$$

$$\Rightarrow \ker T = \text{span} \{ -3x + x^2 \}.$$

In particular, $\dim \ker T = 1$.

Notice, in this example $T: P_2 \rightarrow \mathbb{R}^3$

$$\dim \ker T + \dim \text{Im} T = 1 + 2 = 3$$

And also $\dim P_2 = 3$. This is no accident.

Theorem: Let $T: V \rightarrow W$ be any linear transformation.

Then

$$\dim \ker T + \dim \text{Im} T = \dim V.$$

Pf: Let $n = \dim V$, $k = \dim \ker T$.

Start with a basis $\{u_1, \dots, u_k\}$ for $\ker T$.

Extend it to a basis $\{u_1, \dots, u_k, v_1, \dots, v_{n-k}\}$ for V .

Claim: $\{T(v_1), \dots, T(v_{n-k})\}$ is a basis
for $\text{Im} T$.

Proof of claim: Let $w \in \text{Im } T$. So, there is $v \in V$
 s.t. $T(v) = w$. Since $\{u_1, \dots, u_k, v_1, \dots, v_{n-k}\}$ is a
 basis for V we can find $\lambda_1, \dots, \lambda_k, \mu_1, \dots, \mu_{n-k}$ s.t.

$$v = \lambda_1 u_1 + \dots + \lambda_k u_k + \mu_1 v_1 + \dots + \mu_{n-k} v_{n-k}.$$

Apply T :

$$\begin{aligned} w = T(v) &= \sum_{i=1}^k \lambda_i T(u_i) + \sum_{j=1}^{n-k} \mu_j T(v_j) \\ &= \vec{0} + \sum_{j=1}^{n-k} \mu_j T(v_j). \end{aligned}$$

This shows that $w \in \text{span}\{T(v_j)\}_{j=1}^{n-k}$.

It remains to prove $\{T(v_j)\}_{j=1}^{n-k}$ is lin. independent.

Suppose $\sum_{j=1}^{n-k} a_j T(v_j) = \vec{0}$. We can write as:

$$\sum_{j=1}^{n-k} T(a_j v_j)$$

$$\parallel$$

$$T\left(\sum_{j=1}^{n-k} a_j v_j\right)$$

$$\Rightarrow \sum_{j=1}^{n-k} a_j v_j \in \ker T.$$

But, since $\{u_1, \dots, u_k\}$ is basis for $\ker T$, we

can find b_1, \dots, b_k s.t.

$$\sum_{j=1}^{n-k} a_j v_j = \sum_{i=1}^k b_i u_i.$$

$$\Rightarrow - \sum_{i=1}^k b_i u_i + \sum_{j=1}^{n-k} a_j v_j = \vec{0}$$

But, since $\{u_1, \dots, u_k, v_1, \dots, v_{n-k}\}$ is lin. ind.

$$\Rightarrow b_1 = b_2 = \dots = b_k = a_1 = a_2 = \dots = a_{n-k} = 0. //$$

This completes the proof since

$$\begin{array}{rcl} \dim V & = & \dim \ker T + \dim \operatorname{Im} T \\ \parallel & & \parallel \\ n & = & k + (n-k). \end{array}$$



- Recall the concept of injective. A function $T: V \rightarrow W$ is injective when $T(x) = T(y) \Leftrightarrow x = y$.

Theorem A linear map $T: V \rightarrow W$ is injective if and only if $\ker T = \{\vec{0}\}$.

Pf ^(\Rightarrow) Suppose T is injective. If $T(x) = \vec{0}$ then observe that $T(x) = T(\vec{0}) = \vec{0}$. Since T is injective we see $x = \vec{0}$. Thus $\ker T = \{\vec{0}\}$.

(\Leftarrow) Suppose $\ker T = \{\vec{0}\}$. If $T(x) = T(y)$ we can use linearity to see $T(x - y) = \vec{0}$. Thus $x - y = \vec{0}$ or $x = y$. □

Theorem: Suppose $T: V \rightarrow W$ and $\dim V = \dim W$.

The following are equivalent:

- 1) T is bijective. (injective and surjective),
- 2) T is injective (equiv. $\ker T = \{\vec{0}\}$).
- 3) T is surjective. So, $\text{Im } T = W$.

Pf: This uses the dimension theorem.

Clearly $1) \Rightarrow 2)$. We show $2) \Rightarrow 3)$. So, let

T be injective. By the first theorem, we know that

$\ker T = \{\vec{0}\}$, or $\dim \ker T = 0$. Thus

$$\dim \ker T + \dim \operatorname{Im} T = \dim V \stackrel{\text{assumption}}{=} \dim W.$$

$$\parallel$$
$$\dim \operatorname{Im} T$$

Thus $\dim \operatorname{Im} T = \dim W$. We also have a

theorem saying if $Z \subset W$ is any subspace with

$\dim Z = \dim W$ then $Z = W$. Thus $\operatorname{Im} T = W$

and hence T is surjective. This shows $2) \Rightarrow 3)$
(and $2) \Rightarrow 1)$.)

Finally, we prove $3) \Rightarrow 1)$.

If T is surjective then reading the dimension

formula in reverse we see $\dim \ker T = 0$.

Thus $\ker T = \{\vec{0}\}$. And hence T is injective. \square